src/logic/leads_to.v
@@ -362,53 +362,23 @@ Proof.
     apply exist_impl_intro. exists G. unseal.
 Qed.
 
-Theorem leads_to_fork {A: Type} (h: A → Σ → Prop)
+Lemma leads_to_exist_intro {A} (Γ: predicate) (φ: A → predicate) q :
+  (∀ x, Γ ⊢ φ x ~~> q) →
+  (Γ ⊢ (∃ x, φ x) ~~> q).
+Proof. unseal. Qed.
+
+(* leads_to_fork is really just transitivity but it captures the idea of a
+simple diverge-reconverge pattern *)
+Lemma leads_to_fork {A: Type} (h: A → Σ → Prop)
   (f: predicate) (p q: Σ → Prop) :
   (f ⊢ ⌜p⌝ ~~> ⌜λ s, ∃ x, h x s⌝) →
   (∀ (x: A), f ⊢ ⌜h x⌝ ~~> ⌜q⌝) →
   (f ⊢ ⌜p⌝ ~~> ⌜q⌝).
 Proof.
   intros Hph Hhq.
-
-  (* [inl false] is the initial state, [inl true] is the final state, and [inr
-  x] is in between *)
-  set (S := (bool + A)%type).
-  set (R (x y: S) :=
-         match y, x with
-         | inl false, inr _ => True
-         | inr _, inl true => True
-         | _, _ => False
-         end).
-  assert (well_founded R) as Hwf.
-  { assert (Acc R (inl true)).
-    { constructor; inversion 1. }
-    assert (∀ x, Acc R (inr x)).
-    { intros; constructor. intros []; simpl; try inversion 1.
-      destruct b; [ eauto | inversion 1 ]. }
-    assert (Acc R (inl false)).
-    { constructor. intros []; inversion 1; auto. }
-    intros []; auto. destruct b; auto.
-  }
-  set (h' (l: S) := match l with
-                    | inl false => p
-                    | inl true => q
-                    | inr x => h x
-                    end).
-
-  apply (lattice_leads_to Hwf h' (inl false) (inl true)); [ done | done | ].
-  intros l Hne.
-
-  destruct l.
-  - destruct b; try congruence; simpl.
-    rewrite -> Hph.
-    apply leads_to_weaken; [ done | ].
-    unseal.
-    intros [x Hx].
-    exists (inr x); auto.
-  - simpl.
-    rewrite -> (Hhq a).
-    apply leads_to_weaken; [ done | ].
-    unseal.
+  erewrite <- leads_to_trans; tla_split; [ apply Hph | ].
+  apply leads_to_exist_intro.
+  intros x. fold (⌜h x⌝). eauto.
 Qed.
 
 End TLA.
